compiler/src/compiler/memory_mapped_ext_calls_compiler.v
@@ -1,5 +1,5 @@
 Require Import Coq.ZArith.ZArith.
-Require Import coqutil.Z.Lia.
+Require Import Coq.micromega.Lia.
 Require Import coqutil.Tactics.fwd.
 Require Import compiler.util.Common.
 Require Import bedrock2.Semantics.
@@ -54,7 +54,7 @@ Definition compile_interact{width: Z}{BW: Bitwidth width}
   (results: list Z)(a: string)(args: list Z): list Instruction :=
   match args with
   | [addr; val] => [compile_store a addr val 0]
-  | [addr] => [compile_load a (List.hd 0 results) addr 0]
+  | [addr] => [compile_load a (List.hd RegisterNames.a0 results) addr 0]
   | _ => [] (* invalid, excluded by ext_spec *)
   end.
 
@@ -65,6 +65,24 @@ Local Arguments Z.modulo : simpl never.
 Local Arguments Z.pow: simpl never.
 Local Arguments Z.sub: simpl never.
 Local Arguments Registers.reg_class.all: simpl never.
+
+Section GetSetRegValid.
+  Context {width: Z} {BW: Bitwidth width} {word: word.word width} {locals: map.map Z word}.
+
+  Lemma getReg_valid: forall x (v: word) regs,
+      valid_register x -> map.get regs x = Some v -> getReg regs x = v.
+  Proof.
+    unfold valid_register, getReg. intros. destruct_one_match.
+    - rewrite H0. reflexivity.
+    - exfalso. lia.
+  Qed.
+
+  Lemma setReg_valid:
+    forall x (v: word) regs, valid_register x -> setReg x v regs = map.put regs x v.
+  Proof.
+    unfold valid_register, setReg. intros. destruct_one_match. 1: reflexivity. exfalso. lia.
+  Qed.
+End GetSetRegValid.
 
 Section MMIO.
   Context {iset: InstructionSet}.
@@ -165,17 +183,16 @@ Section MMIO.
       valid_register a ->
       map.get initialL.(getRegs) a = Some addr ->
       Memory.load_bytes n initialL.(getMem) addr = None ->
-      read_step n initialL.(getLog) addr (fun v mRcv =>
+      read_step n initialL.(getLog) addr (fun val mRcv =>
         forall m' : mem,
         map.split m' (getMem initialL) mRcv ->
+        let v := word.of_Z (LittleEndian.combine n val) in
         mcomp_sat (f tt)
           (withRegs (map.put initialL.(getRegs) x v)
           (updateMetrics (addMetricLoads 1)
           (withLogItem ((map.empty, action, [addr]), (mRcv, [v]))
           (withMem m' initialL)))) post) ->
-      mcomp_sat (Bind (Execute.execute
-           (compile_load action x a 0)) f)
-        initialL post.
+      mcomp_sat (Bind (Execute.execute (compile_load action x a 0)) f) initialL post.
   Proof.
     destruct width_cases as [W | W]; subst width;
     intros; subst action;
@@ -183,6 +200,9 @@ Section MMIO.
     match goal with
     | H: _ |- _ => destruct H as [? | [? | [? | [? ?] ] ] ]; subst n
     end;
+    try lazymatch goal with
+        | H: 32 = 64 |- _ => discriminate H
+        end;
     lazymatch goal with
     | |- context[match ?i with _ => _ end] =>
         let i' := eval hnf in i in change i with i'
@@ -203,9 +223,73 @@ Section MMIO.
     (eapply weaken_read_step; [eassumption | cbv beta]);
     intros; repeat step;
     unfold uInt8ToReg, uInt16ToReg, int32ToReg, uInt32ToReg, int64ToReg, MachineWidth_XLEN;
-    rewrite LittleEndian.combine_split.
-    (* TODO read_step must ensure that 0 <= v < 2 ^ (n * 8), maybe use tuples? *)
-  Admitted.
+    rewrite setReg_valid by assumption;
+    rewrite ?sextend_width_nop by reflexivity;
+    only_destruct_RiscvMachine initialL;
+    cbn -[HList.tuple Memory.load_bytes] in *;
+    try (eapply H; assumption).
+  Qed.
+
+  Lemma go_ext_call_store: forall n action a addr v val mGive mKeep
+                                  (initialL: MetricRiscvMachine) post f,
+      action = "memory_mapped_extcall_write" ++ String.of_nat (n * 8) ->
+      (n = 1%nat \/ n = 2%nat \/ n = 4%nat \/ n = 8%nat /\ width = 64) ->
+      valid_register a ->
+      valid_register v ->
+      map.get initialL.(getRegs) a = Some addr ->
+      map.get initialL.(getRegs) v = Some val ->
+      word.unsigned val < 2 ^ (Z.of_nat n * 8) ->
+      Memory.load_bytes n initialL.(getMem) addr = None ->
+      map.split initialL.(getMem) mKeep mGive ->
+      write_step n initialL.(getLog) addr (LittleEndian.split n (word.unsigned val)) mGive ->
+      mcomp_sat (f tt)
+        (updateMetrics (addMetricStores 1)
+        (withXAddrs (invalidateWrittenXAddrs n addr (getXAddrs initialL))
+        (withLogItem ((mGive, action, [addr; val]),
+                      (map.empty, nil))
+        (withMem mKeep initialL)))) post ->
+      mcomp_sat (Bind (Execute.execute (compile_store action a v 0)) f) initialL post.
+  Proof.
+    destruct width_cases as [W | W]; subst width;
+    intros; subst action;
+    unfold compile_store, Execute.execute;
+    match goal with
+    | H: _ |- _ => destruct H as [? | [? | [? | [? ?] ] ] ]; subst n
+    end;
+    try lazymatch goal with
+        | H: 32 = 64 |- _ => discriminate H
+        end;
+    lazymatch goal with
+    | |- context[match ?i with _ => _ end] =>
+        let i' := eval hnf in i in change i with i'
+    end;
+    cbv iota;
+    unfold ExecuteI.execute, ExecuteI64.execute;
+    eapply go_associativity;
+    (eapply go_getRegister; [ eassumption | eassumption | ]);
+    eapply go_associativity;
+    eapply go_associativity;
+    unfold mcomp_sat, Primitives.mcomp_sat, primitivesParams, Bind, free.Monad_free in *;
+    repeat step;
+    unfold Memory.store_bytes;
+    unfold ZToReg, Utility.add, MachineWidth_XLEN;
+    rewrite word.add_0_r;
+    rewrite_match;
+    unfold nonmem_store;
+    unfold regToInt8, regToInt16, regToInt32, regToInt64, MachineWidth_XLEN;
+    eexists _, _;
+    (split; [eassumption | ]);
+    erewrite getReg_valid by eassumption;
+    (split; [assumption | ]);
+    rewrite LittleEndian.combine_split;
+    only_destruct_RiscvMachine initialL;
+    cbn -[HList.tuple Memory.load_bytes invalidateWrittenXAddrs] in *;
+    rewrite Z.mod_small by (split; [eapply word.unsigned_range|assumption]);
+    rewrite word.of_Z_unsigned;
+    lazymatch goal with
+    | H: free.interp interp_action _ _ _ |- free.interp interp_action _ _ _ => exact H
+    end.
+  Qed.
 
   Lemma compile_ext_call_correct: forall resvars extcall argvars,
       FlatToRiscvCommon.compiles_FlatToRiscv_correctly compile_ext_call compile_ext_call
@@ -235,6 +319,7 @@ Section MMIO.
     - (* load *)
       destruct argvars as [ |addr_reg argvars]. 1: discriminate Hl.
       destruct argvars. 2: discriminate Hl. clear Hl.
+      fwd.
       unfold compile_interact in *. cbn [List.length] in *.
       eapply go_fetch_inst; simpl_MetricRiscvMachine_get_set.
       { reflexivity. }
@@ -245,6 +330,138 @@ Section MMIO.
         all: try exact I.
         destruct width_cases as [W | W]; rewrite W; exact I. }
       eapply go_ext_call_load.
-  Abort.
+      { reflexivity. }
+      { assumption. }
+      { clear -V_resvars.
+        destruct resvars.
+        - cbv. auto.
+        - eapply Forall_inv in V_resvars. cbn.
+          unfold valid_FlatImp_var, valid_register in *. lia. }
+      { unfold valid_FlatImp_var, valid_register in *. lia. }
+      { cbn. unfold map.extends in *. eauto. }
+      { cbn. case TODO. (* TODO memory-mapped extcalls disjoint from memory *) }
+      cbn -[String.append].
+      eapply weaken_read_step. 1: eassumption.
+      cbv beta. intros v mRcv HO mL' Hsp.
+      lazymatch goal with
+      | H: forall _ _, outcome _ _ -> _ |- _ =>
+          specialize H with (1 := HO); destruct H as (l' & Hp & HPost)
+      end.
+      fwd.
+      lazymatch goal with
+      | H: map.split _ mKeep map.empty |- _ => eapply map.split_empty_r in H; subst mKeep
+      end.
+      eassert (sep (eq m) _ initialL_mem) as HM by wcancel_assumption.
+      pose proof HM as HM'.
+      destruct HM' as (mm & mL & D & ? & HmL). subst mm.
+      eapply grow_eq_sep in HM. 2: exact Hsp.
+      unfold mcomp_sat, Primitives.mcomp_sat, primitivesParams, Bind, free.Monad_free.
+      repeat step. unfold goodMachine. cbn -[String.append].
+      repeat match goal with
+             | |- exists _, _  => eexists
+             | |- _ /\ _ => split
+             end.
+      { eapply HPost.
+        move D at bottom. move Hsp at bottom.
+        unfold map.split in D, Hsp|-*. split. 1: reflexivity.
+        apply proj2 in Hsp. destruct D as (? & D). subst initialL_mem.
+        eapply map.disjoint_putmany_l in Hsp. apply (proj1 Hsp). }
+      { reflexivity. }
+      { eapply MapEauto.only_differ_union_l.
+        eapply MapEauto.only_differ_put.
+        cbn. left. reflexivity. }
+      { MetricsToRiscv.solve_MetricLog. }
+      { eapply map.put_extends. eassumption. }
+      { eapply map.forall_keys_put; assumption. }
+      { rewrite map.get_put_diff; eauto. unfold RegisterNames.sp.
+        unfold valid_FlatImp_var in *. lia. }
+      { eapply regs_initialized.preserve_regs_initialized_after_put. assumption. }
+      { reflexivity. }
+      { assumption. }
+      { reflexivity. }
+      { reflexivity. }
+      { wcancel_assumption. }
+      { reflexivity. }
+      { case TODO. (* valid_machine *) }
+    - (* store *)
+      destruct argvars as [ |addr_reg argvars]. 1: discriminate Hl.
+      destruct argvars. 1: discriminate Hl.
+      destruct argvars. 2: discriminate Hl. clear Hl.
+      fwd.
+      unfold compile_interact in *. cbn [List.length] in *.
+      eapply go_fetch_inst; simpl_MetricRiscvMachine_get_set.
+      { reflexivity. }
+      { eapply rearrange_footpr_subset. 1: eassumption. wwcancel. }
+      { wcancel_assumption. }
+      { unfold not_InvalidInstruction, compile_store.
+        repeat destruct nValid as [nValid|nValid]; [..|apply proj1 in nValid]; subst n.
+        all: exact I. }
+      eassert (sep (eq m) _ initialL_mem) as HM by wcancel_assumption.
+      eapply subst_split in HM. 2: eassumption.
+      destruct HM as (mH & mL & D & HmH & HM).
+      destruct HmH as (mKeep' & mGive' & HmH & ? & ?). subst mGive' mKeep'.
+      pose proof (LittleEndian.combine_bound v) as B. rewrite Z.mul_comm in B.
+      assert (2 ^ (Z.of_nat n * 8) <= 2 ^ width). {
+        destruct width_cases as [W | W]; rewrite W;
+          match goal with
+          | H: _ |- _ => destruct H as [? | [? | [? | [? ?] ] ] ]; subst n
+          end;
+          cbv; congruence.
+      }
+      eapply go_ext_call_store with (mKeep := map.putmany mKeep mL) (mGive := mGive).
+      { reflexivity. }
+      { assumption. }
+      { unfold valid_FlatImp_var, valid_register in *. lia. }
+      { unfold valid_FlatImp_var, valid_register in *. lia. }
+      { cbn. unfold map.extends in *. eauto. }
+      { cbn. unfold map.extends in *. eauto. }
+      { rewrite word.unsigned_of_Z_nowrap; lia. }
+      { cbn. case TODO. (* TODO memory-mapped extcalls disjoint from memory *) }
+      { cbn. clear HM.
+        unfold map.split in D, HmH|-*.
+        destruct D as (? & D1). destruct HmH as (? & D2). subst initialL_mem mH.
+        eapply map.disjoint_putmany_l in D1. destruct D1 as (D1a & D1b).
+        split.
+        - rewrite <-2map.putmany_assoc. f_equal. apply map.putmany_comm. exact D1b.
+        - eapply map.disjoint_putmany_l. split. 1: assumption.
+          apply map.disjoint_comm. assumption. }
+      { cbn. rewrite word.unsigned_of_Z_nowrap by lia.
+        rewrite LittleEndian.split_combine. assumption. }
+      lazymatch goal with
+      | HO: outcome _ _, H: forall _ _, outcome _ _ -> _ |- _ =>
+          specialize H with (1 := HO); destruct H as (l' & Hp & HPost)
+      end.
+      fwd.
+      unfold mcomp_sat, Primitives.mcomp_sat, primitivesParams, Bind, free.Monad_free.
+      repeat step. unfold goodMachine. cbn -[String.append].
+      repeat match goal with
+             | |- exists _, _  => eexists
+             | |- _ /\ _ => split
+             end.
+      { eapply HPost.
+        eapply map.split_empty_r. reflexivity. }
+      { reflexivity. }
+      { eapply MapEauto.only_differ_refl. }
+      { MetricsToRiscv.solve_MetricLog. }
+      { eassumption. }
+      { assumption. }
+      { assumption. }
+      { assumption. }
+      { reflexivity. }
+      { case TODO. (* instruction still a subset of invalidated XAddrs *) }
+      { reflexivity. }
+      { reflexivity. }
+      { eenough (sep (eq mKeep) _ (map.putmany mKeep mL)).
+        1: wcancel_assumption.
+        do 2 eexists. do 2 split.
+        3: reflexivity.
+        1: reflexivity.
+        2: wcancel_assumption.
+        clear -mem_ok word_ok D HmH.
+        unfold map.split in *. fwd.
+        eapply map.disjoint_putmany_l in Dp1. apply Dp1. }
+      { reflexivity. }
+      { case TODO. (* valid_machine *) }
+  Qed.
 
 End MMIO.
